lawyer/nonblocking/tokens/om_wfree_inst_tokens.v
@@ -34,22 +34,29 @@ Definition token_safety_spec `{invGS_gen HasNoLc Σ, MethodToken MS Σ}
 (** TODO: add the stuckness bit? *)
 Record WaitFreeSpecToken (MS: gmultiset val) := {
   wfst_is_init_st: cfg heap_lang -> Prop;
+
+  wfst_preG: gFunctors -> Prop;
+  wfst_G: gFunctors -> Prop;
+  wfst_Σ: gFunctors;
+  wfst_subG: forall Σ, subG wfst_Σ Σ -> wfst_preG Σ;
+
   (** for wait-free modules, we expect that invariant doesn't contain OM resources *)
-  wfst_mod_inv {Σ} {hG: heap1GS Σ} {iG: invGS_gen HasNoLc Σ}: iProp Σ;
-  wfst_mod_inv_Pers `{heap1GS Σ, invGS_gen HasNoLc Σ} ::
-    Persistent wfst_mod_inv;
-  wfst_init_mod `{heap1GS Σ, invGS_gen HasNoLc Σ, MethodTokenPre Σ}:
+  wfst_mod_inv {Σ} {hG: heap1GS Σ} {iG: invGS_gen HasNoLc Σ} {wG: wfst_G Σ}:
+    iProp Σ;
+  wfst_mod_inv_Pers `{heap1GS Σ, invGS_gen HasNoLc Σ} {wG: wfst_G Σ} ::
+    Persistent (wfst_mod_inv (wG := wG));
+  wfst_init_mod `{heap1GS Σ, invGS_gen HasNoLc Σ, MethodTokenPre Σ, wfst_preG Σ}:
     forall c (INIT: wfst_is_init_st c),
-      ⊢ hl_phys_init_resource c ={⊤}=∗ wfst_mod_inv ∗ 
-          ∃ (_: MethodToken MS Σ), methods_toks MS;
+      ⊢ hl_phys_init_resource c ={⊤}=∗ ∃ (_: MethodToken MS Σ) (wG: wfst_G Σ), 
+                                     wfst_mod_inv (wG := wG) ∗ methods_toks MS;
   wfst_F: nat;
   wfst_spec:
   forall {M: Model} {EM: ExecutionModel heap_lang M} {Σ} {OHE: OM_HL_Env OP_HL_WF EM Σ}
-    {MT: MethodToken MS Σ},
-    (let _: heap1GS Σ := iem_phys HeapLangEM EM in wfst_mod_inv) ⊢
+    {MT: MethodToken MS Σ} {wG: wfst_G Σ},
+    (let _: heap1GS Σ := iem_phys HeapLangEM EM in wfst_mod_inv (wG := wG) ) ⊢
     [∗ set] m ∈ dom MS, method_spec_token MS wfst_F m;
     
   wfst_safety_spec:
-    ∀ {Σ : gFunctors} `{heap1GS Σ, invGS_gen HasNoLc Σ, MethodToken MS Σ},
-      wfst_mod_inv ⊢ [∗ set] m ∈ dom MS, token_safety_spec m;
+    ∀ {Σ : gFunctors} `{heap1GS Σ, invGS_gen HasNoLc Σ, MethodToken MS Σ} {wG: wfst_G Σ},
+      wfst_mod_inv (wG := wG) ⊢ [∗ set] m ∈ dom MS, token_safety_spec m;
 }.
